examples/mtac/Demo.v
@@ -1,0 +1,23 @@
+Require Import ExtLib.Structures.Monad.
+Require Import MirrorCore.Ext.Expr.
+Require Import mtac.McMtac.
+
+Set Implicit Arguments.
+Set Strict Implicit.
+
+Import MonadNotation.
+Import McMtacNotation.
+
+Definition test (t : expr) : McMtac (option expr) :=
+  mmatch t with
+    | [ App (Func 0 nil) (UVar 0) ] =>> fun x => ret (Some x)
+    \ ret None
+  end%mcmtac.
+
+Let tfs := {| tfenv := 0 ; tftype := tvArr (tvType 0) (tvType 0) |} ::
+           {| tfenv := 0 ; tftype := tvType 0 |} :: nil.
+Let tus : list typ := nil.
+Let tvs := (tvType 0 :: nil).
+Let exp := (App (Func 0 nil) (Var 0)).
+
+Eval compute in runMcMtac tfs tus tvs 10 (test exp).
